% Notes and exercises from Introduction to Real Analysis by DePree and Swartz
% By John Peloquin
\documentclass[letterpaper,12pt]{article}
\usepackage{amsmath,amssymb,amsthm,enumitem,fourier}

\newcommand{\R}{\mathbb{R}}

\newcommand{\bigunion}{\bigcup}

\newcommand{\abs}[1]{|{#1}|}
\newcommand{\pos}[1]{#1^{+}}
\renewcommand{\neg}[1]{#1^{-}}
\renewcommand{\vec}[1]{\boldsymbol{#1}}
\newcommand{\dt}{\,d\!t}

% Theorems
\theoremstyle{plain}
\newtheorem*{thm}{Theorem}
\newtheorem*{prop}{Proposition}

\theoremstyle{definition}
\newtheorem*{exer}{Exercise}

\theoremstyle{remark}
\newtheorem*{rmk}{Remark}

% Meta
\title{Notes and exercises from\\\textit{Introduction to Real Analysis}}
\author{John Peloquin}
\date{}

\begin{document}
\maketitle

\section*{Introduction}
This document contains notes and exercises from~\cite{depree}.

\section*{Chapter~13}
We provide an alternative proof of the forward direction of Theorem~42.
\begin{thm} If \(f:[a,b]\to\R\) is integrable, then
\[\int_a^b f=\lim_{c\to a^+}\int_c^b f\]
\end{thm}
\begin{proof}
Note \(\int_c^b f\)~exists for all \(c\in[a,b]\) by Theorem~21. Now
\begin{align*}
\lim_{c\to a^+}\int_c^b f&=\lim_{c\to a^+}\Bigl[\,\int_a^b f-\int_a^c f\,\Bigr]&&\text{by Theorem~18}\\
	&=\int_a^b f-\lim_{c\to a^+}\int_a^c f&&\\
	&=\int_a^b f-\int_a^a f&&\text{by Theorem~27}\\
	&=\int_a^b f&&\qedhere
\end{align*}
\end{proof}
\begin{rmk}
We used the continuity of the indefinite integral (Theorem~27), which was proved using Henstock's Lemma (Lemma~25). The proof of the forward direction of Theorem~42 in the book unnecessarily repeats some ideas from the proof of Henstock's Lemma. See also the proof of the forward direction of Theorem~14.6 in the book.
\end{rmk}

\section*{Chapter~14}
\begin{exer}[12]
Let \(f:[a,\infty)\to\R\) be continuous and such that the indefinite integral \(F(x)=\int_a^x f\) is bounded. Let \(g:[a,\infty)\to\R\) be nonnegative, decreasing, and differentiable. Then \(\int_a^{\infty}fg\)~exists if either \(\lim_{x\to\infty}g(x)=0\) or \(\int_a^{\infty}f\)~exists.
\end{exer}
\begin{proof}
For \(b\in[a,\infty)\), \(fg\)~is continuous on~\([a,b]\), so \(\int_a^b fg\)~exists (Theorem~13.23). By the fundamental theorem of calculus (Theorem~13.28), \(F'=f\) on~\([a,b]\), so integration by parts (Proposition~13.17) yields
\[\int_a^b fg=\int_a^b F'g=F(b)g(b)-F(a)g(a)-\int_a^b Fg'=F(b)g(b)-\int_a^b Fg'\]
Now \(\lim_{b\to\infty}g(b)\) exists since \(g\)~is decreasing and bounded below by zero. If \(\lim_{b\to\infty}g(b)=0\), then boundedness of~\(F\) implies \(\lim_{b\to\infty}F(b)g(b)=0\). If \(\int_a^\infty f\) exists, then \(\lim_{b\to\infty}F(b)\) exists by the continuity of the indefinite integral at~\(\infty\) (Theorem~6), so \(\lim_{b\to\infty}F(b)g(b)\) exists.

We claim \(\int_a^{\infty}Fg'\) exists. First observe
\[\int_a^{\infty}g'=\lim_{b\to\infty}\int_a^bg'=\lim_{b\to\infty}[g(b)-g(a)]=\lim_{b\to\infty}g(b)-g(a)\]
exists by the continuity of the indefinite integral, the fundamental theorem of calculus, and the limit of~\(g\). Since \(g'\le0\),
\[\int_a^{\infty}\abs{g'}=\int_a^{\infty}-g'=-\int_a^{\infty}g'\]
also exists by linearity of the integral. Write \(\abs{F}\le M\). Then \(\abs{Fg'}\le M\abs{g'}\) and \(\int_a^{\infty}M\abs{g'}=M\int_a^{\infty}\abs{g'}\)~exists, so \(\int_a^{\infty}Fg'\) exists by comparison (Corollary~7).

Finally, by continuity of the indefinite integral twice more,
\[\int_a^{\infty}fg=\lim_{b\to\infty}F(b)g(b)-\int_a^{\infty}Fg'\qedhere\]
\end{proof}
\begin{rmk}
These are just Dirichlet's and Abel's tests for convergence of integrals, which are continuous versions of the corresponding discrete tests for infinite series of numbers (Exercises 4.22 and 4.25) and functions (Exercises 11.36 and 11.37). The proofs are essentially the same in the continuous and discrete cases, except integration by parts replaces summation by parts and absolute integrability replaces absolute convergence.
\end{rmk}
\begin{rmk}
Instead of assuming that \(g\)~is nonnegative and decreasing, we may assume only that \(g\)~is bounded and monotone.
\end{rmk}

\section*{Chapter~15}
\begin{rmk}
In the proof of the general Leibniz differentiation rule for integrals (Corollary~9), to see that \(D_1G\)~is continuous, let \(\vec{v_0}=(x_0,y_0,z_0)\) and \(\vec{v}=(x,y,z)\) and observe that
\begin{align*}
\lim_{\vec{v}\to\vec{v_0}}D_1G(\vec{v})&=\lim_{\vec{v}\to\vec{v_0}}\int_y^z D_1f(x,t)\dt\\
	&=\lim_{\vec{v}\to\vec{v_0}}\Bigl[\,\int_y^{y_0}D_1f(x,t)\dt+\int_{y_0}^{z_0}D_1f(x,t)\dt+\int_{z_0}^z D_1f(x,t)\dt\Bigr]\\
	&=\lim_{\vec{v}\to\vec{v_0}}\int_y^{y_0}\!\!\!D_1f(x,t)\dt+\lim_{\vec{v}\to\vec{v_0}}\int_{y_0}^{z_0}\!\!\!D_1f(x,t)\dt+\lim_{\vec{v}\to\vec{v_0}}\int_{z_0}^z\!D_1f(x,t)\dt\\
	&=\lim_{x\to x_0}\int_{y_0}^{z_0}D_1f(x,t)\dt\tag{1}\\
	&=\int_{y_0}^{z_0}D_1f(x_0,t)\dt\tag{2}\\
	&=D_1G(\vec{v_0})
\end{align*}
where (1)~follows from the continuity of indefinite integrals (Theorem~13.27, see above) and (2)~follows from Theorem~5.\qed
\end{rmk}

\noindent We provide an alternative proof of Proposition~47.
\begin{prop}
Let \(f:\R\to\R\) and let \(\{E_i\}\)~be a family of pairwise disjoint subsets of~\(\R\) over each of which \(f\)~is absolutely integrable. Then \(f\)~is absolutely integrable over \(E=\bigunion_{i=1}^{\infty}E_i\) if and only if \(\sum_{i=1}^{\infty}\int_{E_i}\abs{f}<\infty\), in which case
\[\int_E\abs{f}=\sum_{i=1}^{\infty}\int_{E_i}\abs{f}\quad\text{and}\quad\int_E f=\sum_{i=1}^{\infty}\int_{E_i}f\]
\end{prop}
\begin{proof}
We decompose \(f\)~into positive and negative parts (Proposition~13.40(i)).

Since \(f\)~is absolutely integrable over each~\(E_i\), \(\pos{f}\)~and~\(\neg{f}\) are integrable over each~\(E_i\). Let \(S_n=\bigunion_{i=1}^n E_i\), so \(\{S_n\}\)~is increasing and \(E=\bigunion_{i=1}^{\infty}S_i\). By disjoint additivity (Proposition~12(ii)), \(\pos{f}\)~and~\(\neg{f}\) are integrable over each~\(S_n\) with
\[\int_{S_n}\pos{f}=\sum_{i=1}^n\int_{E_i}\pos{f}\quad\text{and}\quad\int_{S_n}\neg{f}=\sum_{i=1}^n\int_{E_i}\neg{f}\]
By monotone convergence (Proposition~16), \(\pos{f}\)~and~\(\neg{f}\) are integrable over~\(E\), and equivalently \(f\)~is absolutely integrable over~\(E\), if and only if
\[\lim_{n\to\infty}\int_{S_n}\pos{f}=\sum_{i=1}^{\infty}\int_{E_i}\pos{f}<\infty\quad\text{and}\quad\sum_{i=1}^{\infty}\int_{E_i}\neg{f}<\infty\tag{1}\]
in which case
\[\int_E\pos{f}=\sum_{i=1}^{\infty}\int_{E_i}\pos{f}\quad\text{and}\quad\int_E\neg{f}=\sum_{i=1}^{\infty}\int_{E_i}\neg{f}\]
Now if (1)~holds, then
\[\sum_{i=1}^{\infty}\int_{E_i}\abs{f}=\sum_{i=1}^{\infty}\int_{E_i}\bigl[\pos{f}+\neg{f}\bigr]=\int_E\pos{f}+\int_E\neg{f}=\int_E\abs{f}<\infty\]
and similarly
\[\sum_{i=1}^{\infty}\int_{E_i}f=\sum_{i=1}^{\infty}\int_{E_i}\bigl[\pos{f}-\neg{f}\bigr]=\int_E\pos{f}-\int_E\neg{f}=\int_E f\]
Conversely, if \(\sum_{i=1}^{\infty}\int_{E_i}\abs{f}<\infty\), then
\[\sum_{i=1}^n\int_{E_i}\pos{f}\le\sum_{i=1}^n\int_{E_i}\abs{f}\le\sum_{i=1}^{\infty}\int_{E_i}\abs{f}<\infty\]
and similarly for \(\sum_{i=1}^n\int_{E_i}\neg{f}\), so (1)~holds.
\end{proof}

% References
\begin{thebibliography}{0}
\bibitem{depree} DePree, John~D. and Charles W. Swartz. \textit{Introduction to Real Analysis.} Wiley, 1988.
\end{thebibliography}
\end{document}
